# Function Evaluation
#### Problem 1:

**Given Function:**  
$$f(x) = 3 - 5x - 2x^2$$

**(a)** Find \( f(4) \)  
$$f(4) = 3 − 5(4) − 2(4)^2 = 3 − 20 − 32 = \boxed{-49}$$

**(b)** Find \( f(0) \)  
$$f(0) = 3 − 5(0) − 2(0)^2 = 3 − 0 − 0 = \boxed{3}$$

**(c)** Find \( f(-3) \)  
$$f(-3) = 3 − 5(-3) − 2(-3)^2 = 3 + 15 − 18 = \boxed{0}$$

**(d)** Find \( f(6 − t) \)  $$
\begin{align*}
f(6 − t) &= 3 − 5(6 − t) − 2(6 − t)^2 \\
&= 3 − 30 + 5t − 72 + 24t − 2t^2 \\
&= \boxed{-2t^2 + 29t - 99}
\end{align*}$$

**(e)** Find \( f(7 − 4x) \)  
$$\begin{align*}
f(7 − 4x) &= 3 − 5(7 − 4x) − 2(7 − 4x)^2 \\
&= 3 − 35 + 20x − 98 + 112x − 32x^2 \\
&= \boxed{-32x^2 + 132x - 130}
\end{align*}$$

**(f)** Find \( f(x + h) \)  
$$\begin{align*}
f(x + h) &= 3 − 5(x + h) − 2(x + h)^2 \\
&= 3 − 5x − 5h − 2x^2 − 4xh − 2h^2 \\
&= \boxed{-2x^2 − 4xh − 2h^2 − 5x − 5h + 3}
\end{align*}$$

---

#### Problem 2:

**Given Function:**  
$$g(t) = \frac{t}{2t + 6}$$

**(a)** Find \( g(0) \)  
$$g(0) = \frac{0}{2\cdot 0 + 6} = \frac{0}{6} = \boxed{0}$$

**(b)** Find \( g(-3) \)  
$$g(-3) = \frac{-3}{2(-3) + 6} = \frac{-3}{-6 + 6} = \frac{-3}{0} = \boxed{\text{undefined}}$$

**(c)** Find \( g(10) \)  
$$g(10) = \frac{10}{2\cdot10 + 6} = \frac{10}{26} = \boxed{\frac{5}{13}}$$

**(d)** Find \( g(x^2) \)  
$$g(x^2) = \frac{x^2}{2x^2 + 6} = \boxed{\frac{x^2}{2x^2 + 6}}$$

**(e)** Find \( g(t + h) \)  
$$g(t + h) = \frac{t + h}{2t + 2h + 6} = \boxed{\frac{t + h}{2t + 2h + 6}}$$

**(f)** Find \( g(t^2 − 3t + 1) \)  
$$g(t^2 − 3t + 1) = \frac{t^2 − 3t + 1}{2t^2 − 6t + 8} = \boxed{\frac{t^2 − 3t + 1}{2t^2 − 6t + 8}}$$

---

#### Problem 3:

**Given Function:**  
$$h(z) = \sqrt{1 - z^2}$$

**(a)** Find \( h(0) \)  
$$h(0) = \sqrt{1 - 0^2} = \sqrt{1} = \boxed{1}$$

**(b)** Find $( h(-\frac{1}{2}) )$  
$$h\left(-\frac{1}{2}\right) = \sqrt{1 - \left(-\frac{1}{2}\right)^2} = \sqrt{\frac{3}{4}} = \boxed{\frac{\sqrt{3}}{2}}$$

**(c)** Find $( h(\frac{1}{2}) )$  
$$h\left(\frac{1}{2}\right) = \sqrt{1 - \left(\frac{1}{2}\right)^2} = \sqrt{\frac{3}{4}} = \boxed{\frac{\sqrt{3}}{2}}$$

**(d)** Find \( h(9z) \)  
$$h(9z) = \sqrt{1 - (9z)^2} = \boxed{\sqrt{1 - 81z^2}}$$

**(e)** Find \( h(z^2 − 2z) \)  
$$h(z^2 − 2z) = \sqrt{1 - (z^2 - 2z)^2} = \boxed{\sqrt{1 - z^4 + 4z^3 - 4z^2}}$$

**(f)** Find \( h(z + k) \)  
$$h(z + k) = \sqrt{1 - (z + k)^2} = \boxed{\sqrt{1 - z^2 - 2zk - k^2}}$$

---

#### Problem 4:
 **Given Function:**  
$$R(x) = \sqrt{3 + x} - \frac{4}{x + 1}$$

**(a)** Find \( R(0) \)  
$$R(0) = \sqrt{3 + 0} - \frac{4}{0 + 1} = \sqrt{3} - \frac{4}{1} = \boxed{\sqrt{3} - 4}$$

**(b)** Find \( R(6) \)  
$$R(6) = \sqrt{3 + 6} - \frac{4}{6 + 1} = \sqrt{9} - \frac{4}{7} = 3 - \frac{4}{7} = \boxed{\frac{17}{7}}$$

**(c)** Find \( R(-9) \)  
$$R(-9) = \sqrt{3 + (-9)} - \frac{4}{-9 + 1} = \sqrt{-6} - \frac{4}{-8} = \boxed{\text{undefined}}$$

**(d)** Find \( R(x + 1) \)  
$$R(x + 1) = \sqrt{3 + (x + 1)} - \frac{4}{(x + 1) + 1} = \sqrt{x + 4} - \frac{4}{x + 2} = \boxed{\sqrt{x + 4} - \frac{4}{x + 2}}$$

**(e)** Find \( R(x^4 - 3) \)  
$$R(x^4 - 3) = \sqrt{3 + (x^4 - 3)} - \frac{4}{(x^4 - 3) + 1} = \sqrt{x^4} - \frac{4}{x^4 - 2} = \boxed{|x^2| - \frac{4}{x^4 - 2}}$$

**(f)** Find $( R\left(\frac{1}{z} - 1\right) )$
$$R\left(\frac{1}{z} - 1\right) = \sqrt{3 + \left(\frac{1}{z} - 1\right)} - \frac{4}{\left(\frac{1}{z} - 1\right) + 1} = \sqrt{2 + \frac{1}{z}} - \frac{4}{\frac{1}{z}} = \boxed{\sqrt{2 + \frac{1}{z}} - 4z}$$